{
 "cells": [
  {
   "cell_type": "markdown",
   "id": "d9743e5f",
   "metadata": {},
   "source": [
    "# Chain Rule\n",
    "\n",
    "When we have one function inside another function (this is called a composite function), we differentiate using the chain rule. \n",
    "An example of a composite function is $y=\\sin(x^2 + 1)$. \n",
    "There are two functions $\\sin(\\ldots)$ and $x^2+1$. \n",
    "We are applying the $\\sin$ function to $x^2+1$, thus making it a function inside a function, or a composite function. \n",
    "\n",
    "The general form of a composite function is: \n",
    "\n",
    "$$\n",
    "y = f[g(x)],\n",
    "$$\n",
    "\n",
    "where $f$ and $g$ are both functions. \n",
    "In the above example $y=\\sin(x^2+1)$, we would have $f[g(x)] = \\sin[g(x)]$ and $g(x) = x^2+1$. \n",
    "\n",
    "To use the chain rule, we have the following steps: \n",
    "\n",
    "1. Introduce a new variable $u$ to be equal to $g(x)$. \n",
    "2. Substitute $u=g(x)$ into the expression $y=f[g(x)]$, so that $y=f(u)$. \n",
    "3. Find $\\frac{dy}{du}$ and $\\frac{du}{dx}$. \n",
    "4. The derivative $\\frac{dy}{dx}$ can be found by this equation \n",
    "\n",
    "    $$\n",
    "    \\frac{dy}{dx} = \\frac{dy}{du} \\times \\frac{du}{dx}\n",
    "    $$\n",
    "\n",
    "    and then subtitute back into $u=g(x)$. \n",
    "\n",
    "The chain rule can be summerised as: \n",
    "\n",
    "$$\n",
    "\\text{If }y=f[g(x)]\\text{ let }u=g(x)\\text{ hence }y=f[g(x)] = f(u)\\text{ then }\\frac{dy}{dx}=\\frac{dy}{du}\\times\\frac{du}{dx}\n",
    "$$\n",
    "\n",
    "Below, we follow the steps of the chain rule to differentiate $y = sin(x^2 + 1)$. \n",
    "\n",
    "1. Introduce a new variable $u$ to be equal to $g(x)$. For this example, $u = x^2+1$. \n",
    "2. Substitute $u=g(x)$ into the expression $y=f[g(x)]$, so that $y=f(u)$. As $u=x^2+1$, this would make $y = \\sin(u)$.\n",
    "3. Find $\\frac{dy}{du}$ and $\\frac{du}{dx}$. In this example, we have: \n",
    "    \n",
    "    $$\n",
    "    y = \\sin(u) \\Rightarrow \\frac{dy}{du} = \\cos(u)\n",
    "    $$\n",
    "\n",
    "    and \n",
    "\n",
    "    $$\n",
    "    u = x^2 + 1 \\Rightarrow \\frac{du}{dx} = 2x\n",
    "    $$\n",
    "\n",
    "4. The derivative $\\frac{dy}{dx}$ can be found by the equation $\\frac{dy}{dx} = \\frac{dy}{du} \\times \\frac{du}{dx}$ and then substitute back in $u=g(x)$. \n",
    "\n",
    "    $$\n",
    "    \\frac{dy}{dx} = \\cos(u)\\times 2x = 2x\\cos(x^2+1)\n",
    "    $$\n",
    "\n",
    "<hr>\n",
    "\n",
    "Python and `sympy` is able to use the chain rule."
   ]
  },
  {
   "cell_type": "code",
   "execution_count": null,
   "id": "a1c364f6",
   "metadata": {},
   "outputs": [],
   "source": [
    "from sympy import symbols, diff, sin\n",
    "\n",
    "x = symbols('x')\n",
    "\n",
    "diff(sin(x ** 2 + 1))"
   ]
  },
  {
   "cell_type": "markdown",
   "id": "72fd5978",
   "metadata": {},
   "source": [
    "<hr>\n",
    "\n",
    "```{admonition} Example\n",
    ":class: example\n",
    "\n",
    "Differentiate $y=(x^2 + 2)^3$ using the chain rule. \n",
    "\n",
    "*Solution:* We take $u = x^2 + 2$ and therefore $y=u^3$. \n",
    "\n",
    "Then we differentiate each of those to find: \n",
    "\n",
    "$$\n",
    "\\frac{du}{dx} = 2x \\;\\;\\;\\;\\; \\frac{dy}{du} = 3u^2\n",
    "$$\n",
    "\n",
    "- From the chain rule: $\\frac{dy}{dx} = \\frac{dy}{du} \\times \\frac{du}{dx}\n",
    "- Substitute in what we know for $\\frac{dy}{du}$ and $\\frac{du}{dx}$: $\\frac{dy}{dx} = 3u^2 \\times 2x$\n",
    "- Substitute that $u$ is $x^2+2$: $\\frac{dy}{dx} = 6x(x^2+2)^2$. \n",
    "```\n",
    "\n",
    "````{margin}\n",
    "```{note}\n",
    "A faster solution to this example would be to use the laws of logarithms to notice that $\\ln(x^3)=3\\ln(x)$ and then differentiate avoiding the use of the chain rule. \n",
    "```\n",
    "````\n",
    "```{admonition} Example\n",
    ":class: example\n",
    "\n",
    "Given $y=ln(x^3)$, find $\\frac{dy}{dx}$. \n",
    "\n",
    "*Solution:* We take $u=x^3$, which menas that $y = \\ln(u)$. \n",
    "\n",
    "Then differentiate to find that: \n",
    "\n",
    "$$\n",
    "\\frac{du}{dx} = 3x^2 \\;\\;\\;\\;\\; \\frac{dy}{du} = \\frac{1}{u}\n",
    "$$\n",
    "\n",
    "- Find the chain rule: $\\frac{dy}{dx} = \\frac{dy}{du} \\times \\frac{du}{dx}$\n",
    "- We can see that: $\\frac{dy}{dx} = \\frac{1}{u} \\times 3x^2$\n",
    "- Substitute that $u$ is $x^3$: $\\frac{dy}{dx} = \\frac{1}{x^3} \\times 3x^2$ \n",
    "- Simplify further: $\\frac{dy}{Dx} = \\frac{3}{x}$\n",
    "```\n",
    "\n",
    "```{admonition} Example\n",
    ":class: example\n",
    "\n",
    "Differentiate $y=\\cos(e^{2x})$\n",
    "\n",
    "*Solution:* Let $u=e^{2x}$, therefore, $y=\\cos(u)$. \n",
    "\n",
    "Differentiate to find: \n",
    "\n",
    "$$\n",
    "\\frac{du}{dx} = 2e^{2x} \\;\\;\\;\\;\\; \\frac{dy}{du} = -\\sin(u)\n",
    "$$\n",
    "\n",
    "- Using the chain rule: $\\frac{dy}{dx} = \\frac{dy}{du} \\times \\frac{du}{dx}$\n",
    "- We can show that: $\\frac{dy}{dx} = -\\sin(u) \\times 2e^{2x}\n",
    "- Substitute that $u=e^{2x}$ \n",
    "- Simplify further: $\\frac{dy}{dx} = -2e^{2x}\\sin(e^{2x})$. \n",
    "```\n",
    "\n",
    "<hr>\n",
    "\n",
    "We can compute the three examples above with Python as follows: "
   ]
  },
  {
   "cell_type": "code",
   "execution_count": null,
   "id": "e15f8b95",
   "metadata": {},
   "outputs": [],
   "source": [
    "diff((x ** 2 + 2) ** 3)"
   ]
  },
  {
   "cell_type": "code",
   "execution_count": null,
   "id": "705dc6b3",
   "metadata": {},
   "outputs": [],
   "source": [
    "from sympy import log\n",
    "\n",
    "diff(log(x ** 3))"
   ]
  },
  {
   "cell_type": "code",
   "execution_count": null,
   "id": "77e7b0f4",
   "metadata": {},
   "outputs": [],
   "source": [
    "from sympy import cos, exp\n",
    "\n",
    "diff(cos(exp(2 * x)))"
   ]
  },
  {
   "cell_type": "markdown",
   "id": "59d9bec0",
   "metadata": {},
   "source": [
    "<hr>\n",
    "\n",
    "````{margin}\n",
    "```{note}\n",
    "This example if complex since we are using multiple rules.\n",
    "Not all problems will be this hard, but it is important to know how to combine the rules of differentiation. \n",
    "An application of this derivative would be able to find the modal speed of a gas.\n",
    "```\n",
    "````\n",
    "\n",
    "```{admonition} Maxwell Boltzmann Distribution\n",
    ":class: chem\n",
    "\n",
    "The Maxwell Boltzmann distribution is a probability distribution of finding particles at certains speed $v$ in 3-dimensions. It has the form of: \n",
    "\n",
    "$$\n",
    "f(x) = Av^2e^{-Bv^2},\n",
    "$$\n",
    "\n",
    "where $A$ and $B$ are positive constants. \n",
    "Using the chain rule and the product rule, find $\\frac{d}{dv}f(v)$. \n",
    "\n",
    "*Solution:* This example involves two steps, first of all the product rule is required to differentiate the whole thing as $f(v)$ is a product of two functions. \n",
    "The chain rule is also needed to differentiate the exponential. \n",
    "Let's call $P = Av^2$ and $Q = e^{-Bv^2}$, thus making $f(v) = P\\times Q$. \n",
    "From the product rule: \n",
    "\n",
    "$$\n",
    "\\frac{d}{dv}f(v) = P\\frac{dQ}{dv} + Q\\frac{dP}{dv}\n",
    "$$\n",
    "\n",
    "We have $\\frac{dP}{dv} = 2Av$, but we will need to use the chain rule to find $\\frac{dQ}{dv}. \n",
    "\n",
    "We let $u=-Bv^2$, making $Q = e^u$. \n",
    "We can then calculate that $\\frac{du}{dv} = -2Bv$ and that $\\frac{dQ}{du} = e^u$. \n",
    "\n",
    "- From here, the chain rule tells us that: $\\frac{dQ}{dv} = \\frac{dQ}{du} \\times \\frac{du}{dv}$\n",
    "- We put in what we have for $\\frac{dQ}{du}$ and $\\frac{du}{dv}$: $\\frac{dQ}{dv} = e^u \\times (-2Bv)$\n",
    "- Substitute $u = -Bv^2$: $\\frac{dQ}{dv} = -2Bve^{-Bv^2}$\n",
    "\n",
    "This can then be substituted into the previous equation. \n",
    "\n",
    "- This gives us: $\\frac{d}{dv}f(v) = P\\frac{dQ}{dv} + Q\\frac{dP}{dv}$\n",
    "- Substitute in what we have found: $\\frac{d}{dv}f(v) = Av^2(-2Bv\\times e^{Bv^2}) + e^{-Bv^2} \\times 2Av$\n",
    "- This can be simplified: $\\frac{d}{dv}f(v) = -2 ABv^3e^{-Bv^2} + 2Ave^{-Bv^2}$\n",
    "- Take a factor of $2Ave^{-Bv2}$ out: $\\frac{d}{dv}f(v) = 2Ave^{-Bv^2}(1-Bv^2)$\n",
    "```\n",
    "\n",
    "<hr>\n",
    "\n",
    "With Python, this rather complex example is simple to get the solution to. "
   ]
  },
  {
   "cell_type": "code",
   "execution_count": null,
   "id": "60540087",
   "metadata": {},
   "outputs": [],
   "source": [
    "from sympy import simplify\n",
    "\n",
    "A, B, v = symbols('A B v')\n",
    "\n",
    "simplify(diff(A * v ** 2 * exp(-B * v ** 2), v))"
   ]
  }
 ],
 "metadata": {
  "kernelspec": {
   "display_name": "m4c",
   "language": "python",
   "name": "python3"
  },
  "language_info": {
   "codemirror_mode": {
    "name": "ipython",
    "version": 3
   },
   "file_extension": ".py",
   "mimetype": "text/x-python",
   "name": "python",
   "nbconvert_exporter": "python",
   "pygments_lexer": "ipython3",
   "version": "3.11.11"
  }
 },
 "nbformat": 4,
 "nbformat_minor": 5
}
